src/HOL/Imperative_HOL/Imperative_HOL_ex.thy
@@ -6,7 +6,7 @@
 header {* Monadic imperative HOL with examples *}
 
 theory Imperative_HOL_ex
-imports Imperative_HOL "ex/Imperative_Quicksort"
+imports Imperative_HOL "ex/Imperative_Quicksort" "ex/Imperative_Reverse" "ex/Linked_Lists"
 begin
 
 end
