src/HOL/Imperative_HOL/ex/Imperative_Reverse.thy
@@ -1,0 +1,112 @@
+theory Imperative_Reverse
+imports "~~/src/HOL/Imperative_HOL/Imperative_HOL" Subarray
+begin
+
+hide (open) const swap rev
+
+fun swap :: "'a\<Colon>heap array \<Rightarrow> nat \<Rightarrow> nat \<Rightarrow> unit Heap" where
+  "swap a i j = (do
+     x \<leftarrow> nth a i;
+     y \<leftarrow> nth a j;
+     upd i y a;
+     upd j x a;
+     return ()
+   done)"
+
+fun rev :: "'a\<Colon>heap array \<Rightarrow> nat \<Rightarrow> nat \<Rightarrow> unit Heap" where
+  "rev a i j = (if (i < j) then (do
+     swap a i j;
+     rev a (i + 1) (j - 1)
+   done)
+   else return ())"
+
+notation (output) swap ("swap")
+notation (output) rev ("rev")
+
+declare swap.simps [simp del] rev.simps [simp del]
+
+lemma swap_pointwise: assumes "crel (swap a i j) h h' r"
+  shows "get_array a h' ! k = (if k = i then get_array a h ! j
+      else if k = j then get_array a h ! i
+      else get_array a h ! k)"
+using assms unfolding swap.simps
+by (elim crel_elim_all)
+ (auto simp: Heap.length_def)
+
+lemma rev_pointwise: assumes "crel (rev a i j) h h' r"
+  shows "get_array a h' ! k = (if k < i then get_array a h ! k
+      else if j < k then get_array a h ! k
+      else get_array a h ! (j - (k - i)))" (is "?P a i j h h'")
+using assms proof (induct a i j arbitrary: h h' rule: rev.induct)
+  case (1 a i j h h'')
+  thus ?case
+  proof (cases "i < j")
+    case True
+    with 1[unfolded rev.simps[of a i j]]
+    obtain h' where
+      swp: "crel (swap a i j) h h' ()"
+      and rev: "crel (rev a (i + 1) (j - 1)) h' h'' ()"
+      by (auto elim: crel_elim_all)
+    from rev 1 True
+    have eq: "?P a (i + 1) (j - 1) h' h''" by auto
+
+    have "k < i \<or> i = k \<or> (i < k \<and> k < j) \<or> j = k \<or> j < k" by arith
+    with True show ?thesis
+      by (elim disjE) (auto simp: eq swap_pointwise[OF swp])
+  next
+    case False
+    with 1[unfolded rev.simps[of a i j]]
+    show ?thesis
+      by (cases "k = j") (auto elim: crel_elim_all)
+  qed
+qed
+
+lemma rev_length:
+  assumes "crel (rev a i j) h h' r"
+  shows "Heap.length a h = Heap.length a h'"
+using assms
+proof (induct a i j arbitrary: h h' rule: rev.induct)
+  case (1 a i j h h'')
+  thus ?case
+  proof (cases "i < j")
+    case True
+    with 1[unfolded rev.simps[of a i j]]
+    obtain h' where
+      swp: "crel (swap a i j) h h' ()"
+      and rev: "crel (rev a (i + 1) (j - 1)) h' h'' ()"
+      by (auto elim: crel_elim_all)
+    from swp rev 1 True show ?thesis
+      unfolding swap.simps
+      by (elim crel_elim_all) fastsimp
+  next
+    case False
+    with 1[unfolded rev.simps[of a i j]]
+    show ?thesis
+      by (auto elim: crel_elim_all)
+  qed
+qed
+
+lemma rev2_rev': assumes "crel (rev a i j) h h' u"
+  assumes "j < Heap.length a h"
+  shows "subarray i (j + 1) a h' = List.rev (subarray i (j + 1) a h)"
+proof - 
+  {
+    fix k
+    assume "k < Suc j - i"
+    with rev_pointwise[OF assms(1)] have "get_array a h' ! (i + k) = get_array a h ! (j - k)"
+      by auto
+  } 
+  with assms(2) rev_length[OF assms(1)] show ?thesis
+  unfolding subarray_def Heap.length_def
+  by (auto simp add: length_sublist' rev_nth min_def nth_sublist' intro!: nth_equalityI)
+qed
+
+lemma rev2_rev: 
+  assumes "crel (rev a 0 (Heap.length a h - 1)) h h' u"
+  shows "get_array a h' = List.rev (get_array a h)"
+  using rev2_rev'[OF assms] rev_length[OF assms] assms
+    by (cases "Heap.length a h = 0", auto simp add: Heap.length_def
+      subarray_def sublist'_all rev.simps[where j=0] elim!: crel_elim_all)
+  (drule sym[of "List.length (get_array a h)"], simp)
+
+end
